update sampler examples to use the twp

theories/examples/approximate_samplers/approx_higherorder_rejection_sampler.v
@@ -9,47 +9,42 @@ Section spec.
   Local Open Scope R.
   Context `{!ub_clutchGS Σ}.
 
-  Definition sampling_scheme_spec (sampler checker : val) 𝜀factor 𝜀final E : iProp Σ
+  (* Spec for samplers which need to amplify some number of times, and then spend.
+     In particular, this is a spec for bounded samplers. *)
+  Definition bounded_sampling_scheme_spec (sampler checker : val) 𝜀factor 𝜀final E Θ : iProp Σ
     := ((∀ 𝜀,
-          {{{ € 𝜀 }}}
+          [[{ € 𝜀 }]]
             ((Val sampler) #())%E @ E
-          {{{ (v : val), RET v;
-               ((WP ((Val checker) v) @ E {{ λ v', ⌜v' = #true ⌝ }}) ∨
-               (∃ 𝜀', € 𝜀' ∗ ⌜𝜀 <= 𝜀' * 𝜀factor ⌝ ∗ (WP ((Val checker) v) @ E {{ λ v', ⌜v' = #true \/ v' = #false⌝ }})))}}}) ∗
+          [[{ (v : val), RET v;
+               ((WP ((Val checker) v) @ E [{ λ v', ⌜v' = #true ⌝ ∗ Θ v }]) ∨
+               (∃ 𝜀', € 𝜀' ∗ ⌜𝜀 <= 𝜀' * 𝜀factor ⌝ ∗ (WP ((Val checker) v) @ E [{ λ v', ⌜v' = #false⌝ ∨ (⌜v' = #true ⌝ ∗ Θ v)}])))}]]) ∗
         (∀ v : val,
-          {{{ € 𝜀final }}}
+          [[{ € 𝜀final }]]
             ((Val sampler) v) @ E
-          {{{ (v' : val), RET v'; (WP ((Val checker) v') @ E {{ λ v', ⌜v' = #true ⌝ }})}}}))%I.
+          [[{ (v' : val), RET v'; (WP ((Val checker) v') @ E [{ λ v'', ⌜v'' = #true ⌝ ∗ Θ v' }])}]]))%I.
 
-End spec.
+  (* Easier to explain spec.
+     It is allowed to wait arbitrarily long before spending,
+     and thus can wait to spend credit €1. *)
+  Definition sampling_scheme_spec (sampler checker : val) εfactor E Θ : iProp Σ
+    := (∀ ε,
+       [[{ € ε }]]
+            ((Val sampler) #())%E @ E
+       [[{ (v : val), RET v;
+               ((WP ((Val checker) v) @ E [{ λ v', ⌜v' = #true ⌝ ∗ Θ v }]) ∨
+               (∃ ε', € ε' ∗ ⌜ε <= ε' * εfactor ⌝ ∗ (WP ((Val checker) v) @ E [{ λ v', ⌜v' = #false⌝ ∨ (⌜v' = #true ⌝ ∗ Θ v)}])))}]])%I.
 
-
-Section accounting.
-  (** Specification for general (stateful) bounded rejection samplers which makes use of
-      Iris' higher order Hoare triples *)
-  Local Open Scope R.
-  Context `{!ub_clutchGS Σ}.
-
-
-  Program Definition generic_geometric_error (r 𝜀final : nonnegreal) (depth : nat) : nonnegreal
-    := (𝜀final * (mknonnegreal (r ^ depth) _))%NNR.
-  Next Obligation. intros. apply pow_le. by destruct r. Qed.
-
-  Lemma final_generic_geometric_error (r 𝜀final : nonnegreal) : (generic_geometric_error r 𝜀final 0%nat) = 𝜀final.
-  Proof. apply nnreal_ext; by rewrite /generic_geometric_error /= Rmult_1_r. Qed.
-
-  Lemma simpl_generic_geometric_error (r 𝜀final : nonnegreal) (depth : nat) :
-    (not (eq (nonneg r) 0)) ->
-    (nnreal_div (generic_geometric_error r 𝜀final (S depth)) r)%NNR = (generic_geometric_error r 𝜀final  depth).
+  Definition unbounded_scheme_implies_bounded sampler checker (εfactor : nonnegreal) E Θ :
+    ⊢ sampling_scheme_spec sampler checker εfactor E Θ -∗
+      bounded_sampling_scheme_spec sampler checker εfactor nnreal_one E Θ.
   Proof.
-    intros.
-    rewrite /generic_geometric_error /nnreal_div /nnreal_mult.
-    apply  nnreal_ext; simpl.
-    rewrite Rmult_assoc;  apply Rmult_eq_compat_l.
-    rewrite -Rmult_comm -Rmult_assoc Rinv_l; [lra|auto].
+    iIntros "?".
+    iSplitL; iFrame.
+    iIntros (? ?) "!> ?".
+    iExFalso; iApply (ec_spend with "[$]").
+    simpl; lra.
   Qed.
-
-End accounting.
+End spec.
 
 
 Section safety.
@@ -57,12 +52,12 @@ Section safety.
   Context `{!ub_clutchGS Σ}.
 
   (* safety for higher-order bounded rejection samplers *)
-  Lemma ho_bounded_approx_safe (sampler checker : val) (r εfinal : nonnegreal) (depth : nat) E :
+  Lemma ho_bounded_approx_safe (sampler checker : val) (r εfinal : nonnegreal) (depth : nat) E Θ :
     (0 < r < 1) ->
     (0 < εfinal < 1) ->
-    sampling_scheme_spec sampler checker r εfinal E -∗
+    bounded_sampling_scheme_spec sampler checker r εfinal E Θ -∗
     € (generic_geometric_error r εfinal depth) -∗
-    (WP (gen_bounded_rejection_sampler #(S depth) sampler checker) @ E {{ fun v => ∃ v', ⌜ v = SOMEV v' ⌝}})%I.
+    (WP (gen_bounded_rejection_sampler #(S depth) sampler checker) @ E [{ fun v => Θ v }])%I.
   Proof.
     (* initial setup *)
     rewrite /sampling_scheme_spec.
@@ -75,110 +70,93 @@ Section safety.
       { iApply (ec_weaken with "Hcr"); rewrite /generic_geometric_error /=; lra. }
       iIntros (next_sample) "Hcheck_accept".
       wp_pures; wp_bind (checker next_sample)%E.
-      iApply (ub_wp_wand with "Hcheck_accept").
-      iIntros (?) "#->"; wp_pures.
-      iModIntro; iExists next_sample; iFrame; auto.
+      iApply (ub_twp_wand with "Hcheck_accept").
+      iIntros (?) "(#-> & ?)"; wp_pures.
+      iModIntro; iFrame.
     - wp_pures.
       replace (bool_decide _) with false; last (symmetry; apply bool_decide_eq_false; lia).
       wp_pures; wp_bind (sampler #())%E.
       iApply ("Hamplify" $! (generic_geometric_error r εfinal (S depth')) with "Hcr").
-      iIntros (next_sample) "!> [Hcheck_accept|[%ε'(Hcr&%Hε'&Hcheck_reject)]]"; wp_pures.
+      iIntros (next_sample) "[Hcheck_accept|[%ε'(Hcr&%Hε'&Hcheck_reject)]]"; wp_pures.
       + wp_bind (checker next_sample)%V.
-        iApply (ub_wp_wand with "Hcheck_accept").
-        iIntros (?) "#->"; wp_pures.
-        iModIntro; iExists next_sample; iFrame; auto.
+        iApply (ub_twp_wand with "Hcheck_accept").
+        iIntros (?) "(#-> & ?)"; wp_pures.
+        iModIntro; iFrame.
       + wp_bind (checker next_sample)%V.
-        iApply (ub_wp_wand with "Hcheck_reject").
-        iIntros (?) "%Hresult".
+        iApply (ub_twp_wand with "Hcheck_reject").
+        iIntros (?) "Hresult".
         iSpecialize ("IH" with "[Hcr]").
         * iApply (ec_spend_le_irrel with "Hcr").
           rewrite /generic_geometric_error /=.
           apply (Rmult_le_reg_r r); auto.
           by rewrite /generic_geometric_error /=
                      (Rmult_comm r _) -Rmult_assoc in Hε'.
-        * destruct Hresult as [-> | ->].
-          { wp_pures; eauto. }
+        * iDestruct "Hresult" as "[-> | (-> & ?)]".
           { do 2 wp_pure.
             iClear "#".
             replace #((S (S depth')) - 1) with #(S depth'); [| do 2 f_equal; lia].
             iApply "IH". }
+          { wp_pures; eauto. }
   Qed.
 
 
-  (* safety for higher-order unbounded rejection samplers (almost the same proof) *)
-  Lemma ho_ubdd_approx_safe (sampler checker : val) (r εfinal : nonnegreal) (depth : nat) E :
+  (* safety for higher-order unbounded rejection samplers *)
+  Lemma ho_ubdd_approx_safe (sampler checker : val) (r : nonnegreal) (depth : nat) E Θ :
     (0 < r < 1) ->
-    (0 < εfinal < 1) ->
-    sampling_scheme_spec sampler checker r εfinal E -∗
-    ▷ € (generic_geometric_error r εfinal depth) -∗
-    (WP (gen_rejection_sampler sampler checker) @ E {{ fun v => ∃ v', ⌜ v = SOMEV v' ⌝}})%I.
+    sampling_scheme_spec sampler checker r E Θ -∗
+    € (generic_geometric_error r nnreal_one depth) -∗
+    (WP (gen_rejection_sampler sampler checker) @ E [{ fun v => Θ v }])%I.
   Proof.
     rewrite /sampling_scheme_spec.
-    iIntros ([Hr_pos Hr] [Hεfinal_pos Hεfinal]) "(#Hamplify&#Haccept) Hcr".
+    iIntros ([Hr_pos Hr]) "#Hamplify Hcr".
     rewrite /gen_rejection_sampler.
     do 7 wp_pure.
     iInduction depth as [|depth' Hdepth'] "IH".
     - wp_pures; wp_bind (sampler #())%E.
-      wp_apply ("Haccept" with "[Hcr]").
-      { iApply (ec_weaken with "Hcr"); rewrite /generic_geometric_error /=; lra. }
-      iIntros (next_sample) "Hcheck_accept".
-      wp_pures; wp_bind (checker next_sample)%E.
-      iApply (ub_wp_wand with "Hcheck_accept").
-      iIntros (?) "#->"; wp_pures.
-      iModIntro; iExists next_sample; iFrame; auto.
+      iExFalso; iApply (ec_spend with "[$]").
+      rewrite /generic_geometric_error /=; lra.
     - wp_pures.
       wp_pures; wp_bind (sampler #())%E.
-      iApply ("Hamplify" $! (generic_geometric_error r εfinal (S depth')) with "Hcr").
-      iIntros (next_sample) "!> [Hcheck_accept|[%ε'(Hcr&%Hε'&Hcheck_reject)]]"; wp_pures.
+      iApply ("Hamplify" $! (generic_geometric_error r nnreal_one (S depth')) with "Hcr").
+      iIntros (next_sample) "[Hcheck_accept|[%ε'(Hcr&%Hε'&Hcheck_reject)]]"; wp_pures.
       + wp_bind (checker next_sample)%V.
-        iApply (ub_wp_wand with "Hcheck_accept").
-        iIntros (?) "#->"; wp_pures.
-        iModIntro; iExists next_sample; iFrame; auto.
+        iApply (ub_twp_wand with "Hcheck_accept").
+        iIntros (?) "(#-> & ?)"; wp_pures.
+        iModIntro; iFrame.
       + wp_bind (checker next_sample)%V.
-        iApply (ub_wp_wand with "Hcheck_reject").
-        iIntros (?) "%Hresult".
+        iApply (ub_twp_wand with "Hcheck_reject").
+        iIntros (?) "Hresult".
         iSpecialize ("IH" with "[Hcr]").
         * iApply (ec_spend_le_irrel with "Hcr").
           rewrite /generic_geometric_error /=.
           apply (Rmult_le_reg_r r); auto.
           by rewrite /generic_geometric_error /=
                      (Rmult_comm r _) -Rmult_assoc in Hε'.
-        * destruct Hresult as [-> | ->].
-          { wp_pures; eauto. }
+        * iDestruct "Hresult" as "[-> | (-> & ?)]".
           { wp_pure.
             iClear "#".
             replace #((S (S depth')) - 1) with #(S depth'); [| do 2 f_equal; lia].
             iApply "IH". }
+          { wp_pures; eauto. }
   Qed.
 
 
   (** Limiting argument: any amount of credit suffices to show the unbounded sampler is safe *)
-  Lemma ho_ubdd_safe (sampler checker : val) (r εfinal ε : nonnegreal) E :
+  Lemma ho_ubdd_safe (sampler checker : val) (r ε : nonnegreal) E Θ :
     (0 < r < 1) ->
-    (0 < εfinal < 1) ->
     0 < ε ->
-    ⊢ sampling_scheme_spec sampler checker r εfinal E -∗
+    ⊢ sampling_scheme_spec sampler checker r E Θ -∗
       €ε -∗
-      WP gen_rejection_sampler sampler checker @ E {{ v, ∃ v', ⌜ v = SOMEV v' ⌝ }}.
+      WP gen_rejection_sampler sampler checker @ E [{ v, Θ v }].
   Proof.
-    iIntros (? ? ?) "#Hspec Hcr".
-    remember (/ NNRbar_to_real (NNRbar.Finite εfinal) * nonneg ε) as p.
-    assert (Hp : (0 < p)).
-    { rewrite Heqp.
-      apply Rmult_lt_0_compat; try done.
-      apply Rinv_0_lt_compat.
-      by destruct H0. }
-    assert (H' : r < 1); first by destruct H.
-    destruct (error_limit' r H' (mkposreal p Hp)) as [depth Hlim].
-    iApply (ho_ubdd_approx_safe _ _ _ _ depth);[|done|done|];[done|]. (* weird unification order *)
-    iApply (ec_spend_le_irrel with "Hcr").
+    iIntros ([? Hr] Hε) "#Hspec Hcr".
     rewrite /generic_geometric_error /=.
-    apply (Rmult_le_reg_l (/ εfinal)).
-    { apply Rinv_0_lt_compat; by destruct H0. }
-    rewrite /= Heqp in Hlim.
-    rewrite -Rmult_assoc Rinv_l; last lra.
-    rewrite Rmult_1_l.
-    by apply Rlt_le.
+    destruct (error_limit' r Hr (mkposreal (nonneg ε) Hε)) as [d Hlim].
+    iApply (ho_ubdd_approx_safe with "[]"); [eauto| iApply "Hspec" |].
+    iApply (ec_spend_le_irrel with "Hcr").
+    rewrite /generic_geometric_error /= Rmult_1_l.
+    apply Rlt_le.
+    simpl in Hlim; eauto.
   Qed.
 End safety.
 
@@ -216,86 +194,51 @@ Section higherorder_rand.
     - apply not_0_INR; lia.
   Qed.
 
+  Definition rand_sampling_scheme_goal (n' : nat) (v : val) : iProp Σ := ∃ (n : nat), ⌜v = #n /\ (n <= n')%nat⌝.
+
   Lemma rand_sampling_scheme_spec (n' m' : nat) (Hnm : (n' < m')%nat) E :
     ⊢ sampling_scheme_spec
           (λ: "_", rand #m')%V
           (λ: "sample", "sample" ≤ #n')%V
           (err_factor (S n') (S m'))
-          (err_factor (S n') (S m'))
-          E.
+          E
+          (rand_sampling_scheme_goal n').
   Proof.
     Opaque INR.
     rewrite /sampling_scheme_spec.
-    iStartProof; iSplit.
-    - (* sampling rule *)
-      iIntros (ε Φ) "!> Hcr HΦ"; wp_pures.
-      iApply (wp_couple_rand_adv_comp  m' _ _ ε (rand_ε2 n' m' ε) _ with "Hcr").
-      { (* uniform bound *)
-        eexists (nnreal_div ε (err_factor (S n') (S m'))); intros s.
-        rewrite /rand_ε2.
-        case_bool_decide; simpl; [|lra].
-        apply Rmult_le_pos.
-        - by apply cond_nonneg.
-        - apply Rlt_le, Rinv_0_lt_compat, Rmult_lt_0_compat.
-          + apply lt_0_INR. lia.
-          + apply Rinv_0_lt_compat. apply lt_0_INR. lia.
-      }
-
-      { (* series convergence *)
-        by apply sample_err_mean_higherorder. }
-
-      iNext; iIntros (s) "Hcr".
-      iApply "HΦ".
-      destruct (le_gt_dec s n') as [|] eqn:Hdec; [iLeft | iRight].
-      + (* the sample is inbounds, the checker should accept *)
-        wp_pures; iModIntro; iPureIntro.
-        do 2 f_equal; apply bool_decide_true; lia.
-      + (* the sample is out of bounds *)
-        iExists _; iSplitL; first iFrame.
-        iSplit.
-        * (* credit is amplified *)
-          iPureIntro.
-          rewrite /rand_ε2 bool_decide_eq_false_2; last first.
-          { rewrite /not; intros; lia. }
-          rewrite /nnreal_div Rmult_assoc /nnreal_inv; simpl.
-          rewrite Rinv_l; [lra|].
-          apply Rmult_integral_contrapositive; split.
-          -- apply Rgt_not_eq, Rlt_gt, lt_0_INR; lia.
-          -- apply Rinv_neq_0_compat.
-             apply Rgt_not_eq, Rlt_gt, lt_0_INR; lia.
-        * (* sampler rejects *)
-          wp_pures; iModIntro; iPureIntro. right.
-          do 2 f_equal; apply bool_decide_false; lia.
-
-    - (* checking rule *)
-      iIntros (s Φ) "!> Hcr HΦ"; wp_pures.
-      wp_apply (wp_rand_err_list_nat _ m' (seq (S n') ((S m') - (S n')))).
-      iSplitL "Hcr".
-      + (* credit accounting *)
-        iApply (ec_spend_irrel with "Hcr").
-        rewrite /err_factor seq_length /=.
-        apply Rmult_eq_compat_l.
-        do 2 f_equal; lia.
-      + iIntros (s') "%Hs'".
-        iApply "HΦ"; wp_pures.
-        iModIntro; iPureIntro.
-        do 2 f_equal; apply bool_decide_true.
-        rewrite List.Forall_forall in Hs'.
-        specialize Hs' with s'.
-        apply Znot_gt_le.
-        intros Hcont; apply Hs'; last reflexivity.
-        rewrite in_seq.
-        split; first lia.
-        replace (S n' + (S m' - S n'))%nat with (S m') by lia.
-        specialize (fin_to_nat_lt s'); by lia.
-
+    iStartProof.
+    iIntros (ε Φ) "!> Hcr HΦ"; wp_pures.
+    iApply (twp_couple_rand_adv_comp1 m' _ _ ε (rand_ε2 n' m' ε) _ with "Hcr").
+    { by apply sample_err_mean_higherorder. }
+    iIntros (s) "Hcr".
+    iApply "HΦ".
+    destruct (le_gt_dec s n') as [|] eqn:Hdec; [iLeft | iRight].
+    + (* the sample is inbounds, the checker should accept *)
+      wp_pures; iModIntro; iPureIntro.
+      split.
+      { do 2 f_equal; apply bool_decide_true; lia. }
+      { eexists _. split; [by f_equal|done]. }
+    + (* the sample is out of bounds *)
+      iExists _; iSplitL; first iFrame.
+      iSplit.
+      * (* credit is amplified *)
+        iPureIntro.
+        rewrite /rand_ε2 bool_decide_eq_false_2; last first.
+        { rewrite /not; intros; lia. }
+        rewrite /nnreal_div Rmult_assoc /nnreal_inv; simpl.
+        rewrite Rinv_l; [lra|].
+        apply Rmult_integral_contrapositive; split.
+        -- apply Rgt_not_eq, Rlt_gt, lt_0_INR; lia.
+        -- apply Rinv_neq_0_compat.
+           apply Rgt_not_eq, Rlt_gt, lt_0_INR; lia.
+      * (* sampler rejects *)
+        wp_pures; iModIntro; iPureIntro. left.
+        { do 2 f_equal; apply bool_decide_false; lia. }
     Unshelve.
     { rewrite Nat2Z.id; apply TCEq_refl. }
   Qed.
 
 End higherorder_rand.
-
-
 
 
 Section higherorder_flip2.
@@ -321,22 +264,18 @@ Section higherorder_flip2.
     := (fun z => if (flip_is_1 z) then εh else εt).
 
   Lemma flip_amplification (ε1 εh εt : nonnegreal) (Hmean : (εh + εt) = 2 * ε1 ) E :
-    {{{ € ε1 }}}
+    [[{ € ε1 }]]
       rand #1 @ E
-    {{{ v, RET #v; ⌜(v = 0%nat) \/ (v = 1%nat) ⌝ ∗ € (scale_flip ε1 εh εt #v) }}}.
+    [[{ v, RET #v; ⌜(v = 0%nat) \/ (v = 1%nat) ⌝ ∗ € (scale_flip ε1 εh εt #v) }]].
   Proof.
     iIntros (Φ) "Hcr HΦ".
-    iApply (wp_couple_rand_adv_comp 1%nat  _ _ ε1 (ε2_flip1 ε1 εh εt) _ with "Hcr").
-    - (* uniform bound *)
-      exists (εh + εt)%NNR; intros n.
-      rewrite /ε2_flip1.
-      destruct (fin_to_bool n); destruct εt, εh; rewrite /bound /=; lra.
+    iApply (twp_couple_rand_adv_comp1 1%nat  _ _ ε1 (ε2_flip1 ε1 εh εt) _ with "Hcr").
     - (* series mean *)
       rewrite SeriesC_finite_foldr /enum /fin_finite /fin_enum /ε2_flip1 /=.
       rewrite Rplus_0_r -Rmult_plus_distr_l Rplus_comm Hmean /=.
       lra.
     - (* continutation *)
-      iNext. iIntros (n) "Hcr".
+      iIntros (n) "Hcr".
       iApply ("HΦ" $! _); iSplitR.
       + iPureIntro.
         inv_fin n; first (left; done).
@@ -350,85 +289,56 @@ Section higherorder_flip2.
       { apply TCEq_refl. }
   Qed.
 
+  Definition flip2_goal (v : val) : iProp Σ := ⌜v = (#1%nat, #1%nat)%V⌝.
 
   Lemma flip2_sampling_scheme_spec E :
     ⊢ sampling_scheme_spec
           (λ: "_", Pair (rand #1) (rand #1))
           (λ: "sample", (((Fst "sample") = #1) && ((Snd "sample") = #1)))
           (nnreal_div (nnreal_nat 3%nat) (nnreal_nat 4%nat))
-          (nnreal_div (nnreal_nat 3%nat) (nnreal_nat 4%nat))
-          E.
+          E
+          flip2_goal.
   Proof.
     rewrite /sampling_scheme_spec.
-    iStartProof; iSplit.
-    - (* amplification rule *)
-      iIntros (𝜀 Φ) "!> Hcr HΦ"; wp_pures.
-      wp_apply (flip_amplification 𝜀
-                  (nnreal_mult 𝜀 (nnreal_div (nnreal_nat 2) (nnreal_nat 3)))
-                  (nnreal_mult 𝜀 (nnreal_div (nnreal_nat 4) (nnreal_nat 3)))
-                   with "Hcr"); [simpl; lra| ].
+    iStartProof.
+    iIntros (𝜀 Φ) "!> Hcr HΦ"; wp_pures.
+    wp_apply (flip_amplification 𝜀
+                (nnreal_mult 𝜀 (nnreal_div (nnreal_nat 2) (nnreal_nat 3)))
+                (nnreal_mult 𝜀 (nnreal_div (nnreal_nat 4) (nnreal_nat 3)))
+                 with "Hcr"); [simpl; lra| ].
+    iIntros (v) "(%Hv&Hcr)".
+    destruct Hv as [-> | ->].
+    + (* first flip was zero, check is going to false and the second flip doesn't matter. *)
+      wp_bind (rand _)%E; iApply twp_rand; auto.
+      iIntros (v') "_"; wp_pures; iModIntro; iApply "HΦ".
+      iRight; iExists _.
+      iSplitL "Hcr"; [iFrame|].
+      iSplit.
+      * (* credit accounting *)
+        iPureIntro; simpl; lra.
+      * (* step the checker *)
+        wp_pures; case_bool_decide; wp_pures; auto.
+    + (* first flip was 1, we only have 2/3 error so we need to amplify up to 4/3
+          in the case that the second flip is not 1 *)
+      replace (scale_flip 𝜀 _ _ _) with (𝜀 * nnreal_div (nnreal_nat 2) (nnreal_nat 3))%NNR; last first.
+      { rewrite /scale_flip /flip_is_1 /=. by apply nnreal_ext. }
+      remember (𝜀 * nnreal_div (nnreal_nat 2) (nnreal_nat 3))%NNR as 𝜀'.
+      wp_bind (rand #1 )%E.
+      wp_apply (flip_amplification 𝜀' nnreal_zero (nnreal_mult 𝜀' (nnreal_nat 2)) with "Hcr").
+      { simpl. lra. }
       iIntros (v) "(%Hv&Hcr)".
       destruct Hv as [-> | ->].
-      + (* first flip was zero, check is going to false and the second flip doesn't matter. *)
-        wp_bind (rand _)%E; iApply wp_rand; auto.
-        iNext; iIntros (v') "_"; wp_pures; iModIntro; iApply "HΦ".
+      * (* second flip was zero *)
+        wp_pures; iModIntro; iApply "HΦ".
         iRight; iExists _.
         iSplitL "Hcr"; [iFrame|].
         iSplit.
-        * (* credit accounting *)
-          iPureIntro; simpl; lra.
-        * (* step the checker *)
-          wp_pures; case_bool_decide; wp_pures; auto.
-      + (* first flip was 1, we only have 2/3 error so we need to amplify up to 4/3
-            in the case that the second flip is not 1 *)
-        replace (scale_flip 𝜀 _ _ _) with (𝜀 * nnreal_div (nnreal_nat 2) (nnreal_nat 3))%NNR; last first.
-        { rewrite /scale_flip /flip_is_1 /=. by apply nnreal_ext. }
-        remember (𝜀 * nnreal_div (nnreal_nat 2) (nnreal_nat 3))%NNR as 𝜀'.
-        wp_bind (rand #1 )%E.
-        wp_apply (flip_amplification 𝜀' nnreal_zero (nnreal_mult 𝜀' (nnreal_nat 2)) with "Hcr").
-        { simpl. lra. }
-        iIntros (v) "(%Hv&Hcr)".
-        destruct Hv as [-> | ->].
-        * (* second flip was zero *)
-          wp_pures; iModIntro; iApply "HΦ".
-          iRight; iExists _.
-          iSplitL "Hcr"; [iFrame|].
-          iSplit.
-          -- (* credit accounting *)
-            iPureIntro; rewrite Heq𝜀' /=; lra.
-          -- (* step the checker *)
-            wp_pures; auto.
-        * (* both flips are 1, checker should accept *)
-          wp_pures; iModIntro; iApply "HΦ".
-          iLeft; wp_pures; auto.
-
-    - (* credit spending rule *)
-      iIntros (s Φ) "!> Hcr HΦ"; wp_pures.
-      wp_bind (rand #1)%E.
-
-      (* give € 1 to the 0 flip, and € 1/2 to the 1 flip *)
-      wp_apply (flip_amplification
-                  (nnreal_div (nnreal_nat 3) (nnreal_nat 4))
-                  (nnreal_div (nnreal_nat 1) (nnreal_nat 2))
-                  nnreal_one with "Hcr"); [simpl; lra|].
-      iIntros (v') "(%Hv'&Hcr)".
-      destruct Hv' as [-> | ->].
-      + (* first flip is zero: but we can spend € 1 to conclude *)
-        iApply (wp_ec_spend with "Hcr").
-        * rewrite /scale_flip /flip_is_1 /=; lra.
-        * rewrite /to_val; done.
-      +  (* we have € 1/2 so we can make the second flip be 1 too *)
-        wp_bind (rand #1)%E.
-        iApply (wp_rand_err _ _ 0%fin with "[Hcr HΦ]").
-        iSplitL "Hcr". { iApply (ec_spend_irrel with "Hcr"). rewrite /=; lra. }
-        iIntros (v') "%Hv'".
+        -- (* credit accounting *)
+          iPureIntro; rewrite Heq𝜀' /=; lra.
+        -- (* step the checker *)
+          wp_pures; auto.
+      * (* both flips are 1, checker should accept *)
         wp_pures; iModIntro; iApply "HΦ".
-        wp_pures; case_bool_decide; wp_pures; auto.
-        (* we have a contradiction in Hv' and H *)
-        exfalso.
-        rewrite /not in Hv', H.
-        inv_fin v'; first auto.
-        intros v'; inv_fin v'; first auto.
-        intros v'; by apply Fin.case0.
+        iLeft; wp_pures; auto.
   Qed.
 End higherorder_flip2.
