theories/examples/approximate_samplers/approx_higherorder_incremental.v
@@ -1,0 +1,98 @@
+(** * Higher order specification for incremental sampling algorithms *)
+From clutch.ub_logic Require Export ub_clutch ub_rules.
+From clutch Require Export examples.approximate_samplers.approx_sampler_lib.
+From Coquelicot Require Import Series.
+Require Import Lra.
+
+Section incremental_spec.
+  Local Open Scope R.
+  Context `{!ub_clutchGS Σ}.
+
+  (* Ψ : state
+     ξ : error
+     L : progress bound
+   *)
+
+  Definition incr_sampling_scheme_spec (sampler checker : val) (Ψ : nat -> iProp Σ) (ξ : nat -> nonnegreal) L iL E Θ : iProp Σ :=
+    ( (* Either 0 credit or 0 progress => we will sample a value which the checker accepts
+         Allowed to consume (or invalidate Ψ) in this process *)
+      ((€ (ξ 0%nat) ∨ Ψ 0%nat) -∗ WP sampler #() @ E [{ fun s => WP checker (Val s) @ E [{fun v => ⌜v = #true⌝ ∗ Θ s }] }]) ∗
+      (* Given any amount of credit and progress, we can get a sample such that... *)
+     □ (∀ i p, (⌜((S p) <= L)%nat ⌝ ∗ ⌜((S i) < iL)%nat ⌝ ∗ € (ξ (S i)) ∗ Ψ (S p)) -∗
+            WP sampler #() @ E [{ fun s =>
+                   (*...we're done by chance alone, or... *)
+                  (WP checker (Val s) @ E [{fun v => ⌜v = #true⌝ ∗ (Θ s)}]) ∨
+                   (*... we make prgress, and can run the checker on the sample without losing progress, or *)
+                  (€ (ξ (S i)) ∗ Ψ p ∗ (Ψ p -∗ WP checker (Val s) @ E [{fun v => Ψ p ∗ (⌜v = #false⌝ ∨ (⌜v = #true⌝ ∗ Θ s))}])) ∨
+                   (*... we lose progress & amplify error, and can run the checker on the sample without losing progress. *)
+                  (∃ p', ⌜(p' <= L)%nat ⌝ ∗ € (ξ i) ∗ Ψ p' ∗ (Ψ p' -∗ WP checker (Val s) @ E [{fun v => Ψ p' ∗ (⌜v = #false⌝ ∨ (⌜v = #true⌝ ∗ Θ s))}]))}]))%I.
+
+
+  Lemma ho_incremental_ubdd_approx_safe (sampler checker : val) Ψ ξ L E i iL p Θ :
+    ⊢ ⌜(p <= L)%nat ⌝ ∗
+      ⌜(i < iL)%nat ⌝ ∗
+    incr_sampling_scheme_spec sampler checker Ψ ξ L iL E Θ ∗
+    € (ξ i) ∗
+    Ψ p -∗
+    WP (gen_rejection_sampler sampler checker) @ E [{ fun v => Θ v }].
+  Proof.
+    rewrite /incr_sampling_scheme_spec.
+    iIntros "(%Hl&%Hil&(Hfinal&#Hamp)&Hcr&HΨ)".
+    rewrite /gen_rejection_sampler.
+    do 7 wp_pure.
+    iRevert (Hl).
+    iInduction i as [|i'] "IHerror" forall (p).
+    - (* base case for error credits *)
+      iIntros "%Hl".
+      wp_pures.
+      wp_bind (sampler _).
+      wp_apply (ub_twp_wand with "[Hfinal Hcr]"); first (iApply "Hfinal"; iFrame).
+      iIntros (s) "Hcheck"; wp_pures.
+      wp_apply (ub_twp_wand with "Hcheck").
+      iIntros (v) "(-> & HΘ)"; wp_pures.
+      eauto.
+    - (* inductive case for error credits *)
+      iIntros "%Hl".
+      iInduction p as [|p'] "IHp".
+      + (* base case for progress measure *)
+        wp_pures.
+        wp_bind (sampler _).
+        wp_apply (ub_twp_wand with "[Hfinal HΨ]"); first (iApply "Hfinal"; iFrame).
+        iIntros (s) "Hcheck"; wp_pures.
+        wp_apply (ub_twp_wand with "Hcheck").
+        iIntros (v) "(-> & HΘ)"; wp_pures.
+        eauto.
+      + (* Inductive case for progress measure *)
+        wp_pures.
+        wp_bind (sampler _).
+        wp_apply (ub_twp_wand with "[Hamp Hcr HΨ]"); first (iApply "Hamp"; iFrame; eauto).
+        iIntros (s) "[Hluck | [(Hcr&HΨ&Hcheck)|[%p'' (%Hp''&Hcr&HΨ&Hcheck)]]]".
+        * (* luck *)
+          wp_pures.
+          wp_bind (checker _).
+          wp_apply (ub_twp_wand with "Hluck").
+          iIntros (?) "(-> & HΘ)".
+          wp_pures.
+          eauto.
+        * (* progress *)
+          wp_pures.
+          wp_bind (checker _).
+          wp_apply (ub_twp_wand with "[Hcheck HΨ]"); first (iApply ("Hcheck" with "[$]")).
+          iIntros (r) "(HΨ&[-> | (-> & A)])".
+          -- (* not lucky: checker rejects *)
+             wp_pure. iApply ("IHp" with "[] Hfinal Hcr HΨ").
+             iPureIntro. lia.
+          -- (* lucky: checker accepts *)
+             wp_pures. eauto.
+        * (* amplification *)
+          wp_pures.
+          wp_bind (checker _).
+          wp_apply (ub_twp_wand with "[Hcheck HΨ]"); first (iApply ("Hcheck" with "[$]")).
+          iIntros (r) "(HΨ&[-> | (-> & A)])".
+          -- (* not lucky: checker rejects *)
+             assert (HiL' : (i' < iL)%nat) by lia.
+             wp_pure. iApply ("IHerror" $! HiL' with "Hfinal Hcr HΨ"). eauto.
+          -- (* lucky: checker accepts *)
+             wp_pures. eauto.
+    Qed.
+End incremental_spec.
